move more stuff around

src/burrow/locations.v
@@ -82,19 +82,7 @@ Fixpoint pls_of_loc {RI} `{!EqDecision RI} `{!Countable RI}
         set_map (augment (nat_of_leftstep RI r)) (pls_of_loc l)
       ∪ set_map (augment (nat_of_rightstep RI l)) (pls_of_loc r)
   end.
-
-Definition build {RI} `{!EqDecision RI} `{!Countable RI} {M} `{!EqDecision M, !TPCM M}
-    (loc: Loc RI) (cell: Cell M) : Branch M. Admitted.
     
-Lemma build_spec {RI} `{!EqDecision RI} `{!Countable RI} {M} `{!EqDecision M, !TPCM M}
-    (loc: Loc RI) (cell: Cell M)
-  : (∀ pl , pl ∈ pls_of_loc loc -> cell_of_pl (build loc cell) pl = cell). Admitted.
-  
-Lemma build_rest_triv
-        {M} `{!EqDecision M, !TPCM M}
-        {RI} `{!EqDecision RI, !Countable RI}
-    (loc: Loc RI) (cell: Cell M)
-  : (∀ pl , ¬(pl ∈ pls_of_loc loc) -> cell_of_pl (build loc cell) pl = triv_cell). Admitted.
 
 Definition ri_of_nat (RI : Type)
     {M} `{!EqDecision M, !TPCM M}
@@ -157,11 +145,6 @@ Qed.
 Inductive ILoc
 *)
 
-Global Instance build_proper
-    {M} `{!EqDecision M, !TPCM M}
-    {RI} `{!EqDecision RI, !Countable RI, !RefinementIndex M RI}
-  (loc: Loc RI) : Proper ((≡) ==> (≡)) (build loc). Admitted.
-
 Definition pls_of_loc_from_left
     {RI} `{!EqDecision RI, !Countable RI}
   (l r: Loc RI) : gset PathLoc :=
@@ -171,17 +154,6 @@ Definition pls_of_loc_from_right
     {RI} `{!EqDecision RI, !Countable RI}
   (l r: Loc RI) : gset PathLoc :=
   set_map (augment (nat_of_rightstep RI l)) (pls_of_loc r).
-
-Lemma branch_is_trivial_build_triv_cell
-    {M} `{!EqDecision M, !TPCM M}
-    {RI} `{!EqDecision RI, !Countable RI, !RefinementIndex M RI}
-  (loc: Loc RI) : branch_trivial (build loc triv_cell). Admitted.
-
-Lemma build_op
-    {M} `{!EqDecision M, !TPCM M}
-    {RI} `{!EqDecision RI, !Countable RI, !RefinementIndex M RI}
-    (i: Loc RI) (x y: Cell M) : build i (x ⋅ y) ≡ build i x ⋅ build i y.
-Admitted.
 
 Section LocationsLemmas.
 
@@ -516,13 +488,6 @@ Lemma i_value_of_pls_of_loc_from_right
 Proof. unfold pls_of_loc in in_pls. generalize in_pls. clear in_pls.
     rewrite elem_of_map. intro. deex. destruct_ands. unfold augment in H.
     destruct x. inversion H. trivial. Qed.
-
-Lemma node_of_pl_build_eq
-  {M} `{!EqDecision M, !TPCM M} `{!RefinementIndex M RI}
-  (pl1 pl2: PathLoc) (loc l1: Loc RI) (c1: Cell M)
-  (pl1_in: pl1 ∈ pls_of_loc loc)
-  (pl2_in: pl2 ∈ pls_of_loc loc)
-  : node_of_pl (build l1 c1) pl1 ≡ node_of_pl (build l1 c1) pl2. Admitted.
   
 Lemma exists_in_pls_of_loc_from_left
   (gamma1 gamma2: Loc RI)
