src/burrow/building.v
@@ -1,0 +1,52 @@
+From iris.algebra Require Export cmra.
+From iris.algebra Require Import proofmode_classes.
+From iris.prelude Require Import options.
+Require Import Burrow.CpdtTactics.
+Require Import coq_tricks.Deex.
+Require Import Coq.Lists.List.
+
+From stdpp Require Import gmap.
+From stdpp Require Import mapset.
+From stdpp Require Import sets.
+From stdpp Require Import list.
+Require Import Burrow.gmap_utils.
+Require Import Burrow.rollup.
+Require Import Burrow.indexing.
+Require Import Burrow.locations.
+
+Definition build {RI} `{!EqDecision RI} `{!Countable RI} {M} `{!EqDecision M, !TPCM M}
+    (loc: Loc RI) (cell: Cell M) : Branch M. Admitted.
+    
+Lemma build_spec {RI} `{!EqDecision RI} `{!Countable RI} {M} `{!EqDecision M, !TPCM M}
+    (loc: Loc RI) (cell: Cell M)
+  : (∀ pl , pl ∈ pls_of_loc loc -> cell_of_pl (build loc cell) pl = cell). Admitted.
+  
+Lemma build_rest_triv
+        {M} `{!EqDecision M, !TPCM M}
+        {RI} `{!EqDecision RI, !Countable RI}
+    (loc: Loc RI) (cell: Cell M)
+  : (∀ pl , ¬(pl ∈ pls_of_loc loc) -> cell_of_pl (build loc cell) pl = triv_cell). Admitted.
+
+Global Instance build_proper
+    {M} `{!EqDecision M, !TPCM M}
+    {RI} `{!EqDecision RI, !Countable RI, !RefinementIndex M RI}
+  (loc: Loc RI) : Proper ((≡) ==> (≡)) (build loc). Admitted.
+
+Lemma branch_is_trivial_build_triv_cell
+    {M} `{!EqDecision M, !TPCM M}
+    {RI} `{!EqDecision RI, !Countable RI, !RefinementIndex M RI}
+  (loc: Loc RI) : branch_trivial (build loc triv_cell). Admitted.
+
+Lemma build_op
+    {M} `{!EqDecision M, !TPCM M}
+    {RI} `{!EqDecision RI, !Countable RI, !RefinementIndex M RI}
+    (i: Loc RI) (x y: Cell M) : build i (x ⋅ y) ≡ build i x ⋅ build i y.
+Admitted.
+
+Lemma node_of_pl_build_eq
+  {M} `{!EqDecision M, !TPCM M}
+  {RI} `{!EqDecision RI, !Countable RI, !RefinementIndex M RI} `{!RefinementIndex M RI}
+  (pl1 pl2: PathLoc) (loc l1: Loc RI) (c1: Cell M)
+  (pl1_in: pl1 ∈ pls_of_loc loc)
+  (pl2_in: pl2 ∈ pls_of_loc loc)
+  : node_of_pl (build l1 c1) pl1 ≡ node_of_pl (build l1 c1) pl2. Admitted.
